fix: address review comments on naming conventions

Iris/Iris/ProgramLogic/EctxLanguage.lean
@@ -97,28 +97,28 @@ variable [BaseStep Expr State Obs]
     `e₁` and `e₂` reduce under a base step.
   -/
 @[grind, rocq_alias prim_step]
-inductive ContextClosure [EvContext Expr Ectx] [BaseStep Expr State Obs]
+inductive ContextStep [EvContext Expr Ectx] [BaseStep Expr State Obs]
   (obs : List Obs) (eₜ : List Expr) (σ₁ σ₂ : State) :
     Expr → Expr → Prop where
   | intro : ∀ (e₁ e₂) (K : Ectx),
     (e₁, σ₁) -<obs>->ᵇ (e₂,σ₂,eₜ) →
-    ContextClosure obs eₜ σ₁ σ₂ (fill K e₁) (fill K e₂)
+    ContextStep obs eₜ σ₁ σ₂ (fill K e₁) (fill K e₂)
 
 @[match_pattern, rocq_alias Ectx_step']
-abbrev ContextClosure.ofBaseStep [EvContext Expr Ectx] [BaseStep Expr State Obs]
+abbrev ContextStep.ofBaseStep [EvContext Expr Ectx] [BaseStep Expr State Obs]
   {e₁ : Expr} {σ₁ obs e₂ σ₂ eₜ} (K : Ectx) :
     (e₁, σ₁) -<obs>->ᵇ (e₂,σ₂,eₜ) →
-    ContextClosure obs eₜ σ₁ σ₂ (fill K e₁) (fill K e₂) :=
-  (ContextClosure.intro _ _ _ ·)
+    ContextStep obs eₜ σ₁ σ₂ (fill K e₁) (fill K e₂) :=
+  (ContextStep.intro _ _ _ ·)
 
 -- @[rocq_alias Ectx_step]
-abbrev ContextClosure.ofBaseStep' [EvContext Expr Ectx] [BaseStep Expr State Obs]
+abbrev ContextStep.ofBaseStep' [EvContext Expr Ectx] [BaseStep Expr State Obs]
   {e e' e₁ : Expr} {σ₁ obs e₂ σ₂ eₜ} (K : Ectx) :
     fill K e₁ = e →
     fill K e₂ = e' →
     (e₁, σ₁) -<obs>->ᵇ (e₂,σ₂,eₜ) →
-    ContextClosure obs eₜ σ₁ σ₂ e e' := fun
-  | rfl, rfl => (ContextClosure.intro _ _ _ ·)
+    ContextStep obs eₜ σ₁ σ₂ e e' := fun
+  | rfl, rfl => (ContextStep.intro _ _ _ ·)
 
 /-- The primitive reduction step generated from a base step is the context closure of
     the base step.  -/
@@ -127,35 +127,35 @@ instance [BaseStep Expr State Obs] [EvContext Expr Ectx] :
     PrimStep Expr State (List Obs) where
   primStep
   | (e₁, σ₁), obs, (e₂, σ₂, eₜ) =>
-    ContextClosure obs eₜ σ₁ σ₂ e₁ e₂
+    ContextStep obs eₜ σ₁ σ₂ e₁ e₂
 
 @[rocq_alias base_reducible]
-def reducible : Expr × State → Prop
+def Reducible : Expr × State → Prop
 | (e,σ) => ∃ obs e' σ' eₜ, (e,σ) -<obs>->ᵇ (e',σ',eₜ)
 
 @[rocq_alias base_reducible_no_obs]
-def reducibleNoObs : Expr × State → Prop
+def ReducibleNoObs : Expr × State → Prop
 | (e,σ) => ∃ e' σ' eₜ, (e,σ) -<[]>->ᵇ (e',σ', eₜ)
 
 @[rocq_alias base_irreducible]
-def irreducible : Expr × State → Prop
+def Irreducible : Expr × State → Prop
 | (e,σ) => ∀ obs e' σ' eₜ, ¬ (e,σ) -<obs>->ᵇ (e',σ',eₜ)
 
 @[rocq_alias base_stuck]
-def stuck [ToVal Expr Val]: Expr × State → Prop
-| (e,σ) => toVal e = none ∧ irreducible (e,σ)
+def Stuck [ToVal Expr Val]: Expr × State → Prop
+| (e,σ) => toVal e = none ∧ Irreducible (e,σ)
 
 variable {e : Expr}{σ : State}
 
 @[rocq_alias not_base_reducible, grind =]
 theorem not_reducible_iff_irreducible :
-    (¬ reducible (e, σ)) ↔ irreducible (e, σ) := by
-  grind only [reducible, irreducible]
+    (¬ Reducible (e, σ)) ↔ Irreducible (e, σ) := by
+  grind only [Reducible, Irreducible]
 
 @[rocq_alias base_reducible_no_obs_reducible, grind .]
 theorem reducible_of_reducibleNoObs :
-    reducibleNoObs (e, σ) → reducible (e, σ) := by
-  grind only [reducibleNoObs, reducible]
+    ReducibleNoObs (e, σ) → Reducible (e, σ) := by
+  grind only [ReducibleNoObs, Reducible]
 
 end BaseStep
 
@@ -235,11 +235,11 @@ instance : Language Expr State Obs Val where
     grind only [val_stuck, fill_not_val]
 
 @[rocq_alias base_atomic]
-def baseAtomic (a : Language.Atomicity) (e : Expr) : Prop :=
+def BaseAtomic (a : Language.Atomicity) (e : Expr) : Prop :=
     ∀ σ obs e' σ' eₜ,
       (e,σ) -<obs>->ᵇ (e',σ',eₜ) →
       match a with
-      | .WeaklyAtomic => PrimStep.irreducible (e',σ')
+      | .WeaklyAtomic => PrimStep.Irreducible (e',σ')
       | .StronglyAtomic => (toVal e').isSome
 
 variable {e e' e₁ e₂ : Expr} {σ σ' σ₁ σ₂ : State}
@@ -250,8 +250,8 @@ open EvContext in
 @[rocq_alias base_redex_unique]
 theorem base_redex_unique K K' (e e' : Expr) σ σ' :
     fill K e = fill K' e' →
-    reducible (e, σ) →
-    reducible (e', σ') →
+    BaseStep.Reducible (e, σ) →
+    BaseStep.Reducible (e', σ') →
     K = comp K' empty ∧
     e = e' := by
   rintro heq ⟨obs, e₂, σ₂, eₜ, bstep⟩ ⟨obs', e₂', σ₂', eₜ', bstep'⟩
@@ -269,7 +269,7 @@ theorem primStep_of_baseStep {e₁ : Expr}{σ₁ obs e₂ σ₂ eₜ}:
     (e₁, σ₁) -<obs>->ᵇ (e₂, σ₂, eₜ) →
     (e₁, σ₁) -<obs>-> (e₂, σ₂, eₜ) := by
   intros h
-  have := ContextClosure.ofBaseStep empty h
+  have := ContextStep.ofBaseStep empty h
   simpa only [EvContext.fill_empty]
 
 theorem baseStep_of_primStep {e₁ : Expr}{σ₁ obs e₂ σ₂ eₜ}:
@@ -289,92 +289,92 @@ theorem baseStep_iff_primStep_of_subredexesAreValues {e₁ : Expr}{σ₁ obs e�
 
 @[rocq_alias base_step_not_stuck]
 theorem base_step_not_stuck {e : Expr} {σ obs e' σ' eₜ} :
-    (e, σ) -<obs>->ᵇ (e', σ', eₜ) → PrimStep.notStuck (e, σ) :=
+    (e, σ) -<obs>->ᵇ (e', σ', eₜ) → PrimStep.NotStuck (e, σ) :=
   Language.notStuck_of_primStep ∘ primStep_of_baseStep
 
 @[rocq_alias fill_prim_step]
 theorem fill_primStep (K : Ectx) {e : Expr} {σ obs e' σ' eₜ} :
     (e, σ) -<obs>-> (e', σ', eₜ) →
     (fill K e, σ) -<obs>-> (fill K e', σ', eₜ) := fun ⟨e₁, e₂, K₁, pstep⟩ => by
-  have := ContextClosure.ofBaseStep (comp K K₁) pstep
+  have := ContextStep.ofBaseStep (comp K K₁) pstep
   simpa only [EvContext.fill_comp]
 
 @[rocq_alias fill_reducible]
 theorem fill_reducible (K : Ectx) {e : Expr} {σ} :
-    PrimStep.reducible (e, σ) → PrimStep.reducible (fill K e, σ) :=
+    PrimStep.Reducible (e, σ) → PrimStep.Reducible (fill K e, σ) :=
   fun ⟨obs, e', σ', eₜ, h⟩ =>
     ⟨obs, fill K e', σ', eₜ, fill_primStep K h⟩
 
 @[rocq_alias fill_reducible_no_obs]
 theorem reducibleNoObs_fill (K : Ectx) {e : Expr} {σ : State} :
-    PrimStep.reducibleNoObs (e, σ) →
-    PrimStep.reducibleNoObs (fill K e, σ) :=
+    PrimStep.ReducibleNoObs (e, σ) →
+    PrimStep.ReducibleNoObs (fill K e, σ) :=
   fun ⟨e', σ', eₜ, h⟩ =>
     ⟨fill K e', σ', eₜ, fill_primStep K h⟩
 
 @[rocq_alias base_prim_reducible]
 theorem primStep_reducible_of_baseStep_reducible :
-    BaseStep.reducible (e, σ) →
-    PrimStep.reducible (e, σ) := fun ⟨obs, e', σ', eₜ, bstep⟩ =>
+    BaseStep.Reducible (e, σ) →
+    PrimStep.Reducible (e, σ) := fun ⟨obs, e', σ', eₜ, bstep⟩ =>
   ⟨obs, e', σ', eₜ, primStep_of_baseStep bstep⟩
 
 @[rocq_alias base_prim_fill_reducible]
 theorem primStep_reducible_fill_of_baseStep_reducible :
-    BaseStep.reducible (e, σ) →
-    PrimStep.reducible (fill K e, σ) := fun ⟨obs, e', σ', eₜ, bstep⟩ =>
+    BaseStep.Reducible (e, σ) →
+    PrimStep.Reducible (fill K e, σ) := fun ⟨obs, e', σ', eₜ, bstep⟩ =>
   ⟨obs, fill K e', σ', eₜ, .ofBaseStep K bstep⟩
 
 @[rocq_alias base_prim_reducible_no_obs]
 theorem primStep_reducibleNoObs_of_baseStep_reducibleNoObs :
-    BaseStep.reducibleNoObs (e, σ) →
-    PrimStep.reducibleNoObs (e, σ) := fun ⟨e', σ', eₜ, bstep⟩ =>
+    BaseStep.ReducibleNoObs (e, σ) →
+    PrimStep.ReducibleNoObs (e, σ) := fun ⟨e', σ', eₜ, bstep⟩ =>
   ⟨e', σ', eₜ, primStep_of_baseStep bstep⟩
 
 @[rocq_alias base_prim_fill_reducible_no_obs]
 theorem primStep_reducibleNoObs_fill_of_baseStep_reducibleNoObs :
-    BaseStep.reducibleNoObs (e, σ) →
-    PrimStep.reducibleNoObs (fill K e, σ) := fun ⟨e', σ', eₜ, bstep⟩ =>
+    BaseStep.ReducibleNoObs (e, σ) →
+    PrimStep.ReducibleNoObs (fill K e, σ) := fun ⟨e', σ', eₜ, bstep⟩ =>
   ⟨fill K e', σ', eₜ, .ofBaseStep K bstep⟩
 
 @[rocq_alias base_prim_irreducible]
 theorem baseStep_irreducible_of_primStep_irreducible :
-    PrimStep.irreducible (e, σ) →
-    BaseStep.irreducible (e, σ) := fun h obs e' σ' eₜ bstep =>
+    PrimStep.Irreducible (e, σ) →
+    BaseStep.Irreducible (e, σ) := fun h obs e' σ' eₜ bstep =>
   h obs e' σ' eₜ <| primStep_of_baseStep bstep
 
 @[rocq_alias prim_base_reducible]
 theorem baseStep_reducible_of_primStep_reducible :
-    PrimStep.reducible (e, σ) →
+    PrimStep.Reducible (e, σ) →
     SubredexesAreValues e →
-    BaseStep.reducible (e, σ) := fun ⟨obs, e', σ', eₜ, pstep⟩ subredexValues =>
+    BaseStep.Reducible (e, σ) := fun ⟨obs, e', σ', eₜ, pstep⟩ subredexValues =>
   ⟨obs, e', σ', eₜ, baseStep_of_primStep pstep subredexValues⟩
 
 @[rocq_alias prim_base_irreducible]
 theorem primStep_irreducible_of_baseStep_irreducible :
-    BaseStep.irreducible (e, σ) →
+    BaseStep.Irreducible (e, σ) →
     SubredexesAreValues e →
-    PrimStep.irreducible (e, σ) := fun birred subredexValues obs e' σ' eₜ pstep =>
+    PrimStep.Irreducible (e, σ) := fun birred subredexValues obs e' σ' eₜ pstep =>
   birred obs e' σ' eₜ (baseStep_of_primStep pstep subredexValues)
 
 @[rocq_alias base_stuck_stuck]
 theorem primStep_stuck_of_baseStep_stuck :
-    BaseStep.stuck (e, σ) →
+    BaseStep.Stuck (e, σ) →
     SubredexesAreValues e →
-    PrimStep.stuck (e, σ) := fun ⟨toVal_none, birred⟩ subredexValues =>
+    PrimStep.Stuck (e, σ) := fun ⟨toVal_none, birred⟩ subredexValues =>
   ⟨toVal_none, primStep_irreducible_of_baseStep_irreducible birred subredexValues⟩
 
 @[rocq_alias ectx_language_atomic, implicit_reducible]
 def Atomic.ofBaseAtomic (a : Language.Atomicity) :
-    baseAtomic a e →
+    BaseAtomic a e →
     SubredexesAreValues e →
     Language.Atomic a e := fun batomic subredexValues => {
       atomic := fun σ obs e' σ' eₜ pstep =>
-        by grind [baseAtomic]
+        by grind [BaseAtomic]
     }
 
 @[rocq_alias base_reducible_prim_step_ctx]
 theorem exists_baseStep_of_primStep_fill_of_redex_baseStep_reducible :
-    BaseStep.reducible (e₁, σ₁) →
+    Reducible (e₁, σ₁) →
     (fill K e₁, σ₁) -<obs>-> (e', σ₂, eₜ) →
     ∃ e₂, e' = fill K e₂ ∧ (e₁, σ₁) -<obs>->ᵇ (e₂, σ₂, eₜ) := by
   generalize heq : fill K e₁ = e at *
@@ -387,7 +387,7 @@ theorem exists_baseStep_of_primStep_fill_of_redex_baseStep_reducible :
 
 @[rocq_alias base_reducible_prim_step]
 theorem baseStep_of_primStep_of_baseStep_reducible :
-    BaseStep.reducible (e₁, σ₁) →
+    Reducible (e₁, σ₁) →
     (e₁, σ₁) -<obs>-> (e₂, σ₂, eₜ) →
     (e₁, σ₁) -<obs>->ᵇ (e₂, σ₂, eₜ) := fun bred pstep =>
   have ⟨e₂', heq, bstep⟩ := exists_baseStep_of_primStep_fill_of_redex_baseStep_reducible (K := empty) bred (EvContext.fill_empty e₁ ▸ pstep)
@@ -407,13 +407,13 @@ instance (K : Ectx) : Language.Context (fill (Expr := Expr) K) where
     simp only [← EvContext.fill_comp, EvContext.fill_inj, Function.Injective.eq_iff,
       exists_eq_left'] at *
     subst heq
-    exact ContextClosure.ofBaseStep K'' bstep
+    exact ContextStep.ofBaseStep K'' bstep
 
 /-- There is a pure base step between `e₁` and `e₂` if there is a unique base step between
     them which produces no observations nor spawns new threads.  -/
 @[rocq_alias pure_base_step]
 structure PureBaseStep (e₁ e₂ : Expr) : Prop where
-  safe : ∀ σ : State, BaseStep.reducibleNoObs (e₁, σ)
+  safe : ∀ σ : State, ReducibleNoObs (e₁, σ)
   deterministic : ∀ {σ₁ σ₂ : State} {obs e₂' eₜ},
     (e₁, σ₁) -<obs>->ᵇ (e₂', σ₂, eₜ) →
     obs = [] ∧ σ₁ = σ₂ ∧ e₂ = e₂' ∧ eₜ = []
